finish asm call example

theories/proof_techniques.v
@@ -164,75 +164,80 @@ Proof.
 Qed.
 
 (** * tsim *)
-Definition tsim {EV} (mi ms : module EV) (σi : mi.(m_state)) (κss : trace EV) (σs : ms.(m_state)) (Is : list (bool * (mi.(m_state) * ms.(m_state) → Prop))) :=
-  ∀ κs n,
-    Forall (λ '(b, Pσ), ∀ κs n' σi' σs',
-      (if b then n' ⊆ n else tiS n' ⊆ n) →
-      (Pσ : _ → Prop) (σi', σs') →
-      σi' ~{ mi, κs, n' }~>ₜ - →
-      σs' ~{ ms, κs }~>ₜ -) Is →
-    σi ~{ mi, κs, n }~>ₜ - →
+
+Definition tsim {EV} (n : trace_index) (b : bool) (mi ms : module EV) (σi : mi.(m_state)) (κss : trace EV) (σs : ms.(m_state))  :=
+  ∀ κs n',
+    (if b then tiS n' ⊆ n else n' ⊆ n) →
+    σi ~{ mi, κs, n' }~>ₜ - →
     σs ~{ ms, tapp κss κs }~>ₜ -.
 
 
 Lemma tsim_implies_trefines {EV} (mi ms : mod_state EV) :
-  tsim mi ms (mi.(ms_state)) tnil (ms.(ms_state)) [] →
+  (∀ n, tsim n false mi ms (mi.(ms_state)) tnil (ms.(ms_state))) →
   trefines mi ms.
-Proof. move => Hsim. constructor => ? /thas_trace_n [??]. by apply: Hsim; [econs|]. Qed.
+Proof. move => Hsim. constructor => ? /thas_trace_n [??]. by apply: Hsim => /=. Qed.
 
-Lemma tsim_remember {EV} {mi ms : module EV} (Pσ : _ → Prop) σi σs Is :
-  Pσ (σi, σs) →
-  (∀ σi σs, Pσ (σi, σs) → tsim mi ms σi tnil σs ((false, Pσ)::Is)) →
-  tsim mi ms σi tnil σs Is.
+Lemma tsim_mono {EV} {mi ms : module EV} σi σs b n n' κs:
+  tsim n' b mi ms σi κs σs →
+  n ⊆ n' →
+  tsim n b mi ms σi κs σs.
+Proof. move => Hsim Hn ???. apply: Hsim. by destruct b; (etrans; [done|]). Qed.
+
+Lemma tsim_mono_b {EV} {mi ms : module EV} σi σs n κs:
+  tsim n false mi ms σi κs σs →
+  tsim n true mi ms σi κs σs.
+Proof. move => Hsim Hn ??. apply: Hsim. by apply ti_lt_impl_le. Qed.
+
+Definition Plater (P : bool → Prop) : Prop :=
+  P true → P false.
+Arguments Plater _ /.
+
+Lemma tsim_remember {EV} {mi ms : module EV} (Pσ : _ → _ → Prop) σi σs b n :
+  Pσ n (σi, σs) →
+  (∀ n n' σi σs, tiS n' ⊆ n → Pσ n (σi, σs) → Pσ n' (σi, σs)) →
+  (* TODO: can one somehow link this n' to the n? *)
+  (∀ n', Plater (λ b', ∀ σi σs, Pσ n' (σi, σs) → tsim n' b' mi ms σi tnil σs)) →
+  tsim n b mi ms σi tnil σs.
 Proof.
-  move => HP Hsim κs' n Hall Ht /=.
-  elim/ti_lt_ind: n κs' σi σs Hall Ht HP.
-  move => n IHn κs' σi σs Hall Ht HP. apply: Hsim; [done| |done].
-  econs; [|done]. move => ???????.
-  apply: IHn; [done| |done|done].
-  apply: Forall_impl; [done|] => -[b ?] Hb ?????. apply: Hb.
-  destruct b. all: etrans; [done|]; by apply ti_lt_impl_le.
+  move => HP HPmono Hsim κs' n' Hn Ht /=.
+  have {}Hn: n' ⊆ n. { destruct b; (etrans; [|done]) => //. apply ti_le_S. }
+  elim/ti_lt_ind: n n' κs' σi σs Hn HP Ht.
+  move => n IHn n' κs' σi σs Hn HP Ht.
+  apply: Hsim ; [|done|done|done].
+  move => ????? Hn'/=. eapply IHn; [done..|].
+  by apply: HPmono.
 Qed.
 
-Lemma tsim_remember_all {EV A} {mi ms : module EV} σi σs Is :
-  (∀ x, tsim mi ms (σi x) tnil (σs x) ((false, λ σ, ∃ x, σ = (σi x, σs x))::Is)) →
-  ∀ x : A, tsim mi ms (σi x) tnil (σs x) Is.
+Lemma tsim_remember_all {EV A} {mi ms : module EV} σi σs b n:
+  (∀ n, Plater (λ b', ∀ x, tsim n b' mi ms (σi x) tnil (σs x))) →
+  ∀ x : A, tsim n b mi ms (σi x) tnil (σs x).
 Proof.
-  move => Hsim x. apply: (tsim_remember (λ σ, ∃ x, σ = (σi x, σs x))). { naive_solver. }
-  move => ?? [?[??]]. subst. apply: Hsim.
+  move => Hsim x. apply: (tsim_remember (λ _ σ, ∃ x, σ = (σi x, σs x))).
+  all: naive_solver.
 Qed.
 
-Lemma tsim_close_loop {EV} {mi ms : module EV} σi σs Is :
-  Exists (λ '(b, P), b = true ∧ P (σi, σs)) Is →
-  tsim mi ms σi tnil σs Is.
-Proof.
-  move => /Exists_exists [[??][?[??]]] κs n /Forall_forall Hall. subst.
-  apply: (Hall (_, _)); [done| simpl; done |done].
-Qed.
-
-Lemma tsim_step_l {EV} {mi ms : module EV} σi σs Is :
+Lemma tsim_step_l {EV} {mi ms : module EV} σi σs n b :
   (∀ κ Pσi,
       mi.(m_step) σi κ Pσi →
-      ∃ σi', Pσi σi' ∧ tsim mi ms σi' (option_trace κ) σs ((prod_map (const true) id) <$> Is)) →
-  tsim mi ms σi tnil σs Is.
+      ∃ σi', Pσi σi' ∧ tsim n true mi ms σi' (option_trace κ) σs) →
+  tsim n b mi ms σi tnil σs.
 Proof.
-  move => Hsim κs' n HIs /tnhas_trace_inv Ht.
+  move => Hsim κs' n' Hn /tnhas_trace_inv Ht.
   apply: thas_trace_under_tall; [done..|] => {Ht} κs [[??]|[?[?[?[?[?[?[<- ?]]]]]]]]. { tend. }
   have [?[? {}Hsim]]:= Hsim _ _ ltac:(done).
   apply: Hsim. 2: { naive_solver. }
-  eapply Forall_fmap, Forall_impl; [done|] => -[b ?] /= Hall ?????. apply: Hall.
-  destruct b.
-  - etrans; [done|]. apply ti_lt_impl_le. etrans; [|done]. econs. by econs.
-  - etrans; [|done]. econs. etrans; [done|]. by econs.
+  destruct b; (etrans; [|done]).
+  - econs. apply ti_lt_impl_le. etrans; [|done]. econs. by econs.
+  - etrans; [|done]. econs. by econs.
     Unshelve. done.
 Qed.
 
-Lemma tsim_step_r {EV} {mi ms : module EV} σi σs Is κs κs' κs'' :
+Lemma tsim_step_r {EV} {mi ms : module EV} σi σs n b κs κs' κs'' :
   κs = tapp κs' κs'' →
-  σs ~{ ms, κs' }~>ₜ (λ σs', tsim mi ms σi κs'' σs' Is) →
-  tsim mi ms σi κs σs Is.
+  σs ~{ ms, κs' }~>ₜ (λ σs', tsim n b mi ms σi κs'' σs') →
+  tsim n b mi ms σi κs σs.
 Proof.
-  move => -> Hsim κss n HIs Ht. rewrite -assoc_L. apply: thas_trace_trans; [done|] => ? {}Hsim.
+  move => -> Hsim κss n' HIs Ht. rewrite -assoc_L. apply: thas_trace_trans; [done|] => ? {}Hsim.
   by apply: Hsim.
 Qed.
 
@@ -240,38 +245,38 @@ Create HintDb tsim discriminated.
 Global Hint Constants Opaque : tsim.
 Global Hint Variables Opaque : tsim.
 Class TSimStepI {EV} (mi : module EV) (σi : mi.(m_state)) (P : (option EV → mi.(m_state) → Prop) → Prop) : Prop := {
-  tsim_stepi_proof ms σs Is κ Pσi:
+  tsim_stepi_proof ms σs n κ Pσi:
     mi.(m_step) σi κ Pσi →
-    P (λ κ σi', tsim mi ms σi' (option_trace κ) σs Is) →
-    ∃ σi', Pσi σi' ∧ tsim mi ms σi' (option_trace κ) σs Is
+    P (λ κ σi', tsim n true mi ms σi' (option_trace κ) σs) →
+    ∃ σi', Pσi σi' ∧ tsim n true mi ms σi' (option_trace κ) σs
 }.
 Global Hint Mode TSimStepI + + ! - : tsim.
 
-Lemma tsim_step_i {EV} (mi : module EV) σi P `{!TSimStepI mi σi P} ms σs Is :
-  P (λ κ σi', tsim mi ms σi' (option_trace κ) σs (prod_map (const true) id <$> Is)) →
-  tsim mi ms σi tnil σs Is.
+Lemma tsim_step_i {EV} (mi : module EV) σi P `{!TSimStepI mi σi P} ms σs n b:
+  P (λ κ σi', tsim n true mi ms σi' (option_trace κ) σs) →
+  tsim n b mi ms σi tnil σs.
 Proof. move => HP. apply tsim_step_l => ???. by apply tsim_stepi_proof. Qed.
 
 Class TSimStepS {EV} (ms : module EV) (σs : ms.(m_state)) (κs : trace EV)
       (P : (trace EV → ms.(m_state) → Prop) → Prop) : Prop := {
-  tsim_steps_proof mi σi Is:
-    P (λ κs' σs', tsim mi ms σi κs' σs' Is) →
-    ∃ κs' κs'', κs = tapp κs' κs'' ∧ σs ~{ ms, κs' }~>ₜ (λ σs', tsim mi ms σi κs'' σs' Is)
+  tsim_steps_proof mi σi n b:
+    P (λ κs' σs', tsim n b mi ms σi κs' σs') →
+    ∃ κs' κs'', κs = tapp κs' κs'' ∧ σs ~{ ms, κs' }~>ₜ (λ σs', tsim n b mi ms σi κs'' σs')
 }.
 Global Hint Mode TSimStepS + + ! + - : tsim.
 
-Lemma tsim_step_s {EV} (ms : module EV) σs κs P `{!TSimStepS ms σs κs P} mi σi Is :
-  P (λ κs' σs', tsim mi ms σi κs' σs' Is) →
-  tsim mi ms σi κs σs Is.
+Lemma tsim_step_s {EV} (ms : module EV) σs κs P `{!TSimStepS ms σs κs P} mi σi n b :
+  P (λ κs' σs', tsim n b mi ms σi κs' σs') →
+  tsim n b mi ms σi κs σs.
 Proof.
   revert select (TSimStepS _ _ _ _) => -[Hproof]. move => /Hproof [?[?[??]]]. subst.
   by apply: tsim_step_r.
 Qed.
 
 Ltac tsim_step_s :=
-  notypeclasses refine (tsim_step_s _ _ _ _ _ _ _ _); [solve [typeclasses eauto with tsim]|]; simpl.
+  notypeclasses refine (tsim_step_s _ _ _ _ _ _ _ _ _); [solve [typeclasses eauto with tsim]|]; simpl.
 Ltac tsim_step_i :=
-  notypeclasses refine (tsim_step_i _ _ _ _ _ _ _); [solve [typeclasses eauto with tsim]|]; simpl.
+  notypeclasses refine (tsim_step_i _ _ _ _ _ _ _ _); [solve [typeclasses eauto with tsim]|]; simpl.
 
 
 (** * proving a refinement based on another refinement *)
