theories/asm.v
@@ -318,8 +318,8 @@ Module asm_examples.
   Lemma asm_mul_refines_itree :
     trefines (MS asm_module (initial_asm_state asm_mul)) (MS (mod_itree _ _) (itree_mul, tt)).
   Proof.
-    apply tsim_implies_trefines => /=. rewrite /initial_asm_state. move: (∅) => rs.
-    move: rs. apply tsim_remember_all => rs.
+    apply tsim_implies_trefines => /= n. rewrite /initial_asm_state. move: (∅) => rs.
+    move: rs. apply tsim_remember_all => {}n Hloop rs.
     tsim_step_i => pc i rs' HPC Hi.
     rewrite {1}/itree_mul. rewrite unfold_forever. rewrite -/itree_mul.
 
@@ -346,7 +346,7 @@ Module asm_examples.
     tsim_step_i => ??. rewrite {1}/asm_mul. simplify_map_eq.
     tsim_step_s. tsim_step_s. split. { by rewrite insert_insert. }
     tsim_step_s. tsim_step_s.
-    rewrite -/itree_mul. apply tsim_close_loop. left. naive_solver.
+    apply Hloop.
   Qed.
 
   Definition asm_mul_client : gmap Z asm_instr :=
@@ -378,12 +378,12 @@ Module asm_examples.
 
   Definition itree_mul_client : itree (moduleE asm_event unit) unit :=
     (rec-fix f _ :=
-       b ← translate (inr_) (TAll bool);;;
-       if b then Ret ()
-       else
        pc ← translate (inr_) (TExist Z);;;
        rs ← translate (inr_) (TExist _);;;
        translate (inr_) (TVis (ERecvJump pc rs));;;;
+       (* The env can choose if this call should be treated as a call or a return. *)
+       b ← translate (inr_) (TAll bool);;;
+       if b then Ret (pc, rs) else
        if bool_decide (pc = 200) then
          translate (inr_) (TAssume (is_Some (rs !! "R1")));;;;
          translate (inr_) (TAssume (is_Some (rs !! "R2")));;;;
@@ -391,10 +391,7 @@ Module asm_examples.
          r30 ← translate (inr_) (TAssumeOpt (rs !! "R30"));;;
          r29' ← translate (inr_) (TExist Z);;;
          translate (inr_) (TVis (EJump 100 (<["PC":=100]> $ <["R30":= 212]> $ <["R29":= r29']> $ <["R2":= 2]> $ <["R1":= 2]> $ rs)));;;;
-         f ();;;;
-         pc' ← translate (inr_) (TExist Z);;;
-         rs' ← translate (inr_) (TExist _);;;
-         translate (inr_) (TVis (ERecvJump pc' rs'));;;;
+         '(pc', rs') ← f ();;;
          translate (inr_) (TAssume (pc' = 212));;;;
          translate (inr_) (TAssume (is_Some (rs' !! "R30")));;;;
          translate (inr_) (TAssume (rs' !! "R29" = Some r29'));;;;
@@ -409,69 +406,23 @@ Module asm_examples.
        else translate (inr_) TNb
     ) ();;;; TUb.
 
-    Lemma itree_step_recursive_bind_s EV S R Q A B (f : A → itree (callE A B +' _) _) (t : itree (moduleE EV S) R) (k : R → itree (_ +' moduleE EV S) Q) h s κs:
-      TSimStepS (mod_itree EV S) (x ← interp (recursive f) (ITree.bind (translate inr_ t) k);;; h x, s) κs
-            (λ G, G κs ((ITree.bind t (fun r => x ← interp (recursive f) (k r);;; h x)), s)).
-    Proof.
-      constructor => ????. eexists tnil, _. split; [done|].
-      apply itree_rel_intro. rewrite interp_bind bind_bind interp_translate /= interp_trigger_h.
-      tend => ? <-. done.
-    Qed.
-    Global Hint Resolve itree_step_recursive_bind_s : tsim.
-    Lemma itree_step_recursive_s EV S R A B (f : A → itree (callE A B +' _) _) (t : itree (moduleE EV S) R) h s κs:
-      TSimStepS (mod_itree EV S) (x ← interp (recursive f) (translate inr_ t);;; h x, s) κs
-            (λ G, G κs ((x ← t;;; h x), s)).
-    Proof.
-      constructor => ????. eexists tnil, _. split; [done|].
-      apply itree_rel_intro. rewrite interp_translate /= interp_trigger_h.
-      tend => ? <- /=. done.
-    Qed.
-    Global Hint Resolve itree_step_recursive_s : tsim.
-    Lemma itree_step_interp_ret_s EV S R E  (f : E ~> itree (moduleE EV S)) (a : R) h s κs:
-      TSimStepS (mod_itree EV S) (x ← interp f (Ret a);;; h x, s) κs (λ G, G κs (h a, s)).
-    Proof.
-      constructor => ????. eexists tnil, _. split; [done|].
-      apply itree_rel_intro. rewrite interp_ret bind_ret_l. tend => ? <-. done.
-    Qed.
-    Global Hint Resolve itree_step_interp_ret_s : tsim.
-
-  Lemma tsim_remember_rec {EV S A B} {mi : module EV} σi r (h : B → _) Is s:
-    (∀ x y, tsim mi (mod_itree EV S) (σi x) tnil (h y, s x) Is) →
-    (∀ x h',
-       (∀ x y, tsim mi (mod_itree EV S) (σi x) tnil (h' y, (s x)) Is) →
-       tsim mi (mod_itree EV S) (σi x) tnil ((y ← rec r ();;; h' y), (s x))
-       ((false, λ σ, ∃ x h',
-          σ = (σi x, ((y ← rec r ();;; h' y), s x)) ∧
-          ∀ x y, tsim mi (mod_itree EV S) (σi x) tnil (h' y, s x) Is)::Is)) →
-    ∀ x : A, tsim mi (mod_itree EV S) (σi x) tnil ((y ← rec r ();;; h y), s x) Is.
-  Proof.
-    move => Hh Hsim x.
-    eapply (tsim_remember (ms:=mod_itree _ _)
-      (λ σ, ∃ x h', σ = (σi x, ((y ← rec r ();;; h' y), s x)) ∧
-          ∀ x y, tsim mi (mod_itree EV S) (σi x) tnil (h' y, s x) Is)). { naive_solver. }
-    move => ?? [?[?[[??]?]]]. subst.
-    by apply: Hsim.
-  Qed.
-
-  Lemma tsim_drop_loop {EV} {mi ms : module EV} σi σs κs Is :
-    tsim mi ms σi κs σs [] →
-    tsim mi ms σi κs σs Is.
-  Proof. move => Hsim κs' n _. by apply: Hsim. Qed.
 
   Lemma asm_mul_client_refines_itree :
     trefines (MS asm_module (initial_asm_state asm_mul_client)) (MS (mod_itree _ _) (itree_mul_client, tt)).
   Proof.
-    apply tsim_implies_trefines => /=. rewrite /initial_asm_state. move: (∅) => rs.
+    apply tsim_implies_trefines => /= n. rewrite /initial_asm_state. move: (∅) => rs.
     rewrite {1}/itree_mul_client /rec_fix. set rc := (X in (rec X)).
-    move: rs. apply tsim_remember_rec. { move => ??. rewrite -(bind_ret_r TUb). by tsim_step_s. }
-    move => rs CONT HCONT.
+    move: rs. apply (tsim_remember_rec (mi:=asm_module) (λ σi '(pc, rs) s',
+          ∃ i, σi = AsmState (Some i) rs asm_mul_client ∧ rs !! "PC" = Some pc ∧ asm_mul_client !! pc = Some i)).
+    { move => ????. rewrite -(bind_ret_r TUb). by tsim_step_s. }
+    move => {}n Hloop rs CONT HCONT.
     rewrite {1}rec_as_interp {2}/rc.
-    tsim_step_s. tsim_step_s => -[].
-    { tsim_step_s. apply: tsim_drop_loop. apply: HCONT. }
     tsim_step_i => pc i rs' HPC Hi.
     tsim_step_s. tsim_step_s. eexists _.
     tsim_step_s. tsim_step_s. eexists _.
     tsim_step_s. tsim_step_s. split; [done|].
+    tsim_step_s. tsim_step_s => -[].
+    { tsim_step_s. apply tsim_mono_b. apply HCONT. naive_solver. }
     move: Hi. rewrite !lookup_insert_Some !lookup_empty => Hi. destruct_all!; simplify_eq.
     all: repeat (rewrite bool_decide_false; [done|]); rewrite bool_decide_true //.
     all: try by tsim_step_s; tsim_step_s.
@@ -500,15 +451,8 @@ Module asm_examples.
       f_equal. apply map_eq => i. apply option_eq => ?.
       rewrite !lookup_insert_Some. naive_solver.
     }
-    (* tsim_step_s. *)
 
-    rewrite interp_bind interp_recursive_call.
-    tsim_step_s. apply tsim_close_loop. left. split; [done|]. eexists _, _. split; [done|].
-    move => rs'' ?.
-    tsim_step_i => pc' i rs''' HPC' Hi'.
-    tsim_step_s. tsim_step_s. eexists _.
-    tsim_step_s. tsim_step_s. eexists _.
-    tsim_step_s. tsim_step_s. split; [done|].
+    tsim_step_s. apply Hloop => ? [pc' rs''] [] [i [? [HPC' Hi']]].
     tsim_step_s. tsim_step_s => ?.
     unfold asm_mul_client in Hi'. simplify_map_eq.
     tsim_step_s. tsim_step_s => -[r30'' HR30''].
@@ -526,6 +470,6 @@ Module asm_examples.
     tsim_step_s. tsim_step_s. split. { f_equal. by rewrite insert_insert. }
 
     rewrite interp_recursive_call.
-    apply tsim_close_loop.
+    apply Hloop => ???. apply HCONT.
   Qed.
 End asm_examples.
